theories/examples.v
@@ -325,6 +325,10 @@ Proof.
     + econstructor => //.
       move => k ty; rewrite list_lookup_singleton_Some.
       case => _ <-; by constructor.
+    + econstructor => //.
+      move => i ty.
+      rewrite list_lookup_singleton_Some => [[? <-]].
+      by constructor.
     + by apply has_fields_ROBox.
     + by set_solver.
     + move => f fty arg.
@@ -342,6 +346,7 @@ Proof.
   }
   eapply SeqTy.
   { eapply NewTy with (targs := []).
+    + by econstructor.
     + by econstructor.
     + by apply has_fields_IntBoxS.
     + by set_solver.
@@ -1087,12 +1092,97 @@ Proof.
   by rewrite /wf_cdef_constraints_bounded /= Forall_nil.
 Qed.
 
+Lemma wf_parent_ok : map_Forall (λ _cname, wf_cdef_parent_ok) Δ.
+Proof.
+  rewrite map_Forall_lookup => c0 d0.
+  rewrite lookup_insert_Some.
+  case => [[? <-]|[?]].
+  { by rewrite /wf_cdef_parent_ok . }
+  rewrite lookup_insert_Some.
+  case => [[? <-]|[?]].
+  { by rewrite /wf_cdef_parent_ok. }
+  rewrite lookup_insert_Some.
+  case => [[? <-]|[?]].
+  { rewrite /wf_cdef_parent_ok /=.
+    econstructor => //.
+    rewrite /σ => i ty.
+    rewrite list_lookup_singleton_Some => [[? <-]].
+    by constructor.
+  }
+  rewrite lookup_singleton_Some.
+  case => [? <-].
+  by rewrite /wf_cdef_parent_ok.
+Qed.
+
+Lemma wf_constraints_ok : map_Forall (λ _cname, wf_cdef_constraints_ok) Δ.
+Proof.
+  rewrite map_Forall_lookup => c0 d0.
+  rewrite lookup_insert_Some.
+  case => [[? <-]|[?]].
+  { rewrite /wf_cdef_constraints_ok; by constructor. }
+  rewrite lookup_insert_Some.
+  case => [[? <-]|[?]].
+  { rewrite /wf_cdef_constraints_ok; by constructor. }
+  rewrite lookup_insert_Some.
+  case => [[? <-]|[?]].
+  { rewrite /wf_cdef_constraints_ok; by constructor. }
+  rewrite lookup_singleton_Some.
+  case => [? <-].
+  rewrite /wf_cdef_constraints_ok; by constructor.
+Qed.
+
+Lemma wf_methods_ok : map_Forall (λ _cname, cdef_methods_ok) Δ.
+Proof.
+  rewrite map_Forall_lookup => c0 d0.
+  rewrite lookup_insert_Some.
+  case => [[? <-]|[?]].
+  { rewrite /cdef_methods_ok /ROBox /=.
+    apply map_Forall_singleton.
+    rewrite /mdef_ok /Get /=.
+    split; last by constructor.
+    by apply map_Forall_empty.
+  }
+  rewrite lookup_insert_Some.
+  case => [[? <-]|[?]].
+  { rewrite /cdef_methods_ok /Box /=.
+    rewrite map_Forall_lookup => x mx.
+    rewrite lookup_insert_Some.
+    case => [[? <-]|[?]].
+    * rewrite /mdef_ok /BoxSet /=.
+      split; last by constructor.
+      apply map_Forall_singleton.
+      by constructor.
+    * rewrite lookup_insert_Some.
+      case => [[? <-]|[?]]; last by rewrite lookup_empty.
+      rewrite /mdef_ok /Get /=.
+      split; first by apply map_Forall_empty.
+      by constructor.
+  }
+  rewrite lookup_insert_Some.
+  case => [[? <-]|[?]].
+  { rewrite /cdef_methods_ok /IntBoxS /=.
+    apply map_Forall_singleton.
+    rewrite /mdef_ok /IntBoxSSet /=.
+    split; last by constructor.
+    apply map_Forall_singleton.
+    by constructor.
+  }
+  rewrite lookup_insert_Some.
+  case => [[? <-]|[?]]; last by rewrite lookup_empty.
+  rewrite /cdef_methods_ok /Main /=.
+  apply map_Forall_singleton.
+  split; last by constructor.
+  by apply map_Forall_empty.
+Qed.
+
 Lemma wf: wf_cdefs Δ.
 Proof.
   split.
   by apply wf_extends_wf.
   by apply wf_parent.
+  by apply wf_parent_ok.
   by apply wf_constraints_wf.
+  by apply wf_constraints_ok.
   by apply wf_constraints_bounded.
   by apply wf_override.
   by apply wf_fields.
@@ -1102,6 +1192,7 @@ Proof.
   by apply wf_methods_bounded.
   by apply wf_methods_wf.
   by apply wf_methods_mono.
+  by apply wf_methods_ok.
   by apply wf_mdefs.
   by apply wf_mono.
 Qed.
@@ -1126,7 +1217,11 @@ Proof.
   apply (@step_updN_soundness sem_heapΣ n).
   iMod sem_heap_init as (Hheap) "Hmain" => //.
   iModIntro.
-  iDestruct ((cmd_adequacy interp_env_empty _ _ _ wf wfinit ht _ _ _ he) with "Hmain") as "H" => /=.
+  assert (Σcoherency : Σinterp [] []) by done.
+  assert (wfΣc : Forall wf_constraint []).
+  { rewrite Forall_forall => ?. by set_solver. }
+  assert (wfΣi : interp_env_as_mixed [] []) by done.
+  iDestruct ((cmd_adequacy [] [] _ _ _ wf wfinit wfΣc wfΣi Σcoherency ht _ _ _ he) with "Hmain") as "H" => /=.
   iRevert "H".
   iApply updN_mono.
   iIntros "[Hh [Hthis Hl]]".
@@ -1156,7 +1251,11 @@ Proof.
   apply (@step_updN_soundness sem_heapΣ n).
   iMod sem_heap_init as (Hheap) "Hmain" => //.
   iModIntro.
-  iDestruct ((cmd_adequacy interp_env_empty _ _ _ wf wfinit ht _ _ _ he) with "Hmain") as "H" => /=.
+  assert (Σcoherency : Σinterp [] []) by done.
+  assert (wfΣc : Forall wf_constraint []).
+  { rewrite Forall_forall => ?. by set_solver. }
+  assert (wfΣi : interp_env_as_mixed [] []) by done.
+  iDestruct ((cmd_adequacy [] [] _ _ _ wf wfinit wfΣc wfΣi Σcoherency ht _ _ _ he) with "Hmain") as "H" => /=.
   iRevert "H".
   iApply updN_mono.
   iIntros "[Hh [_ Hl]]".
