theories/lang.v
@@ -8,12 +8,6 @@ From stdpp Require Import base strings gmap stringmap fin_maps.
 (* Not using iris but importing their ssreflect dependencies *)
 From iris.proofmode Require Import tactics.
 
-(* TODO:
- * - maybe update definitions of bounded and gen_targs to take
- *   a variance list or a class definition as input, and some
- *   of the details away.
- *)
-
 (* Helper tactics *)
 Ltac inv H := inversion H; subst; clear H.
 
@@ -362,6 +356,8 @@ Inductive visibility := Public | Private.
 
 (* S <: T *)
 Definition constraint := (lang_ty * lang_ty)%type.
+
+Definition bounded_constraint n c := bounded n c.1 ∧ bounded n c.2.
 
 Record classDef := {
   classname: tag;
